linearization_ext_tmp2.v

proofs/compiler/linearization_ext_tmp2.v
@@ -1362,18 +1362,18 @@ with forget_imed_cmd (fn0: funname) (pl0 pl1: plinfo)
 
 Require Import Equality. 
 
-Definition forget_imed_i_ok_stat (i: instr) :=
+Definition forget_imed_i_ok_statm (i: instr) :=
   forall (fn0: funname) (pl0: plinfo),
     let X := imed_i fn0 i pl0 in
     projT1 X = fst (forget_imed_i (projT2 X)).
 
-Definition forget_imed_cmd_ok_stat (c: cmd) :=
+Definition forget_imed_cmd_ok_statm (c: cmd) :=
   forall (fn0: funname) (pl0: plinfo),
     let X := imed_cmd fn0 c pl0 in
     projT1 X = fst (forget_imed_cmd (projT2 X)).
 
-Lemma forget_imed_i_ok (i: instr) : forget_imed_i_ok_stat i.
-  unfold forget_imed_i_ok_stat.
+Lemma forget_imed_i_ok (i: instr) : forget_imed_i_ok_statm i.
+  unfold forget_imed_i_ok_statm.
   intros.
   destruct pl0; simpl.
   destruct (imed_i fn0 i (n,l)); simpl.
@@ -1403,8 +1403,8 @@ Lemma forget_imed_i_ok (i: instr) : forget_imed_i_ok_stat i.
   }
 Qed.  
 
-Lemma forget_imed_cmd_ok (c: cmd) : forget_imed_cmd_ok_stat c.
-  unfold forget_imed_cmd_ok_stat.
+Lemma forget_imed_cmd_ok (c: cmd) : forget_imed_cmd_ok_statm c.
+  unfold forget_imed_cmd_ok_statm.
   intros.
   destruct pl0; simpl.
   destruct (imed_cmd fn0 c (n,l)); simpl.
@@ -1414,28 +1414,28 @@ Lemma forget_imed_cmd_ok (c: cmd) : forget_imed_cmd_ok_stat c.
   destruct (@forget_imed_cmd _ _ _ _); simpl; auto.
 Qed.
   
-Definition imed_i_correct_stat (i: instr) :=
+Definition imed_i_correct_statm (i: instr) :=
   forall (fn0: funname) (pl0: plinfo),
     linear_l2r_i fn0 i pl0 = forget_imed_i (projT2 (imed_i fn0 i pl0)).
 
-Definition imed_cmd_correct_stat (c: cmd) :=
+Definition imed_cmd_correct_statm (c: cmd) :=
   forall (fn0: funname) (pl0: plinfo),
      linear_l2r_c linear_l2r_i fn0 c pl0 = 
      forget_imed_cmd (projT2 (imed_cmd fn0 c pl0)).
 
-Lemma imed_correct (i: instr) : imed_i_correct_stat i.
+Lemma imed_correct (i: instr) : imed_i_correct_statm i.
 Proof.
-  set Pi := imed_i_correct_stat.
-  set Pi_r := fun i => forall ii, imed_i_correct_stat (MkI ii i).
-  set Pc := imed_cmd_correct_stat.
+  set Pi := imed_i_correct_statm.
+  set Pi_r := fun i => forall ii, imed_i_correct_statm (MkI ii i).
+  set Pc := imed_cmd_correct_statm.
   set IP := instr_Rect (Pr := Pi_r) (Pi := Pi) (Pc := Pc).
   subst Pi Pi_r Pc.
   eapply IP; clear IP.
   { intros. eapply H. }
-  { unfold imed_cmd_correct_stat; simpl.
+  { unfold imed_cmd_correct_statm; simpl.
     intros fn0 [n0 lbl0]; simpl; auto.
   }
-  { unfold imed_i_correct_stat, imed_cmd_correct_stat.
+  { unfold imed_i_correct_statm, imed_cmd_correct_statm.
     intros i0 c H H0 fn0 [n0 lbl0]; simpl.
     clear i.
     specialize (H fn0 (n0, lbl0)); simpl in *.
@@ -1465,109 +1465,15 @@ Proof.
     simpl in A2.
     rewrite A2; auto.
   }
-  { unfold imed_i_correct_stat; simpl; intros; auto. }
-  { unfold imed_i_correct_stat; simpl; intros.
+  { unfold imed_i_correct_statm; simpl; intros; auto. }
+  { unfold imed_i_correct_statm; simpl; intros.
     destruct (oseq.omap lexpr_of_lval xs); simpl; auto.
     destruct (oseq.omap _ _); simpl; auto.
   }
-  { unfold imed_i_correct_stat; simpl; intros; auto. }
+  { unfold imed_i_correct_statm; simpl; intros; auto. }
   
 Admitted.   
     
-
-(* alternative version (probably not useful, just more verbose) *)
-Fixpoint forgetA_imed_i
-  (fn0: funname) (plI plF: plinfo)
-  (tl: LTree fn0 plI plF) : (plinfo * lcmd) :=
-  let LC : (forall (fn0: funname) (pl0 pl1: plinfo)
-                   (tl: LTreeList fn0 pl0 pl1), (plinfo * lcmd)) :=
-    forgetA_imed_cmd in 
-  match tl with
-  | LErrLeaf pl => (pl, nil)
-  | LLeaf pl li => (incrP1 pl, [:: li])
-  | LLeafL pl li => (incrPL1 pl, [:: li ])
-  | LIf1Node pl0 pl1 la_cond0 tl1 la_lbl0 =>
-      let (_, lcm1) := LC fn0 (incrPL1 pl0) pl1 tl1 in  
-      (incrP1 pl1, la_cond0 :: (lcm1 ++ [:: la_lbl0]))
-  | LIfNode pl0 pl1 pl2 la_cond0 tl2 la_goto01 la_lbl0 tl1 la_lbl01 =>
-      let (_, lcm2) := LC _ _ _ tl2 in  
-      let (_, lcm1) := LC _ _ _ tl1 in  
-      (incrP1 pl2, la_cond0 :: (lcm2 ++
-                           la_goto01 :: la_lbl0 ::
-                           (lcm1 ++ [:: la_lbl01])))
-  | LWhileTNode pl0 pl1 pl2 _ la_lbl0 tl1 tl2 la_goto0 =>
-      let (_, lcm1) := LC _ _ _ tl1 in  
-      let (_, lcm2) := LC _ _ _ tl2 in  
-      (incrP1 pl2, la_lbl0 :: (lcm1 ++ (lcm2 ++ [:: la_goto0])))
-  | LWhileFNode pl0 pl1 tl1 =>
-      let (_, lcm1) := LC _ _ _ tl1 in   
-      (pl1, lcm1)
-  | LWhile1Node pl0 pl1 _ la_lbl0 tl1 la_cond0 =>
-      let (_, lcm1) := LC _ _ _ tl1 in  
-      (incrP1 pl1, la_lbl0 :: (lcm1 ++ [:: la_cond0]))
-  | LWhileNode pl0 pl1 pl2 _ la_goto0 la_lbl01 tl2 la_lbl0 tl1 la_cond01 =>
-      let (_, lcm2) := LC _ _ _ tl2 in  
-      let (_, lcm1) := LC _ _ _ tl1 in  
-      (incrP1 pl2, la_goto0 :: la_lbl01 :: (lcm2 ++
-                           (la_lbl0 :: (lcm1 ++ [:: la_cond01]))))
-  | LCallNode pl0 nb na fn' la_before la_after la_call la_ret =>
-      let lbl1 := next_lbl (snd pl0) in
-      let n1 := S (fst pl0 + nb) in
-      ((n1 + na, lbl1), la_before ++ (la_call :: la_ret :: la_after))      
-  end
-with forgetA_imed_cmd (fn0: funname) (plI plF: plinfo)
-  (tl: LTreeList fn0 plI plF) : (plinfo * lcmd) :=
-  match tl with
-  | LListNil pl => (pl, nil)
-  | LListCons pl0 pl1 pl2 t0 tl0 => 
-      let (pl01, lcm1) := @forgetA_imed_i _ pl0 pl1 t0 in
-      let (pl02, lcm2) := @forgetA_imed_cmd _ pl1 pl2 tl0 in
-      (pl2, lcm1 ++ lcm2)
-(*      if (pl1 == pl01) && (pl2 == pl02) then
-      (pl2, lcm1 ++ lcm2) else (plI, nil) *)
-  end.              
-
-Definition forgetA_imed_i_ok_stat (i: instr) :=
-  forall (fn0: funname) (pl0: plinfo),
-    let X := imed_i fn0 i pl0 in
-    projT1 X = fst (forgetA_imed_i (projT2 X)).
-
-Definition forgetA_imed_cmd_ok_stat (c: cmd) :=
-  forall (fn0: funname) (pl0: plinfo),
-    let X := imed_cmd fn0 c pl0 in
-    projT1 X = fst (forgetA_imed_cmd (projT2 X)).
-
-(* same proof as before, not very interesting *)
-Lemma forgetA_imed_ok (i: instr) : forgetA_imed_i_ok_stat i.
-  unfold forgetA_imed_i_ok_stat.
-  intros.
-  destruct pl0; simpl.
-  destruct (imed_i fn0 i (n,l)); simpl.
-  destruct x; simpl.
-  destruct l0; simpl; eauto.
-  { destruct (forgetA_imed_cmd _); simpl; auto. }
-  { set X := (@forgetA_imed_cmd _ _ _ _).
-    destruct X; simpl.
-    set X := (@forgetA_imed_cmd _ _ _ _).
-    destruct X; simpl; auto.
-  }
-  { set X := (@forgetA_imed_cmd _ _ _ _).
-    destruct X; simpl.
-    set X := (@forgetA_imed_cmd _ _ _ _).
-    destruct X; simpl; auto.
-  }
-  { set X := (@forgetA_imed_cmd _ _ _ _).
-    destruct X; simpl; auto.
-  }  
-  { set X := (@forgetA_imed_cmd _ _ _ _).
-    destruct X; simpl; auto.
-  }
-  { set X := (@forgetA_imed_cmd _ _ _ _).
-    destruct X; simpl.
-    set X := (@forgetA_imed_cmd _ _ _ _).
-    destruct X; simpl; auto.
-  }
-Qed.  
 
 
 End FUN.
